testdata/cue/definitions/dyndef_dynfield_concrete_key.cue
@@ -1,0 +1,2 @@
+#K: {kind: "fixed", (kind): "m"}
+out: #K
